# Waves Review

## Important Concepts
- Speed is a property of the medium 
- Wavelength and Amplitude are inversely proportional, as on goes up the other goes down
- Wavelength and frequency are inversely proportional
- Sound in the doppler effect is constant, but the wavelength is longer than stationary when moving away, but shorter when moving toward you. Think of it as the wave being stetched out and compressed
$\lambda_{n} = \frac{4L}{n}$
## Important Formulas
$$
\begin{align}
v = f \cdot \lambda \\ \\
F_{o} = F_{s} \cdot \left[  \frac{V \pm V_{o}}{V \pm V_{s}} \right] && \text{Doppler Effect}\\  \\
L = \frac{n\cdot \lambda_{n}}{2} && \text{Length of a standing wave}\\ \\
\lambda_{n} = \frac{2l}{n} && \text{Wavelength n}\\  \\
f_{1} = \frac{\left( \sqrt{ \frac{T}{\frac{m}{L}} } \right)}{2L} && \text{Tension of a wave on a string}\\  \\
F_{b} = F_{1} - F_{2} && beats\\  \\
v = \sqrt{ \frac{Y}{\rho} } && \text{Speed of sound in solids(Y = young's modulus)} \\ \\
v = \sqrt{ \frac{B}{\rho} } && \text{Speed of sound in fluids(B = bulk modulus)}\\ \\
\Delta L = n\lambda && \text{Constructive Interference}\\ \\
\Delta L = \left( n+\frac{1}{2} \right)\lambda && \text{Destructive Interference}\\  \\

\end{align}
$$


# Standing Waves on String

 L = $\frac{n*\lambda_n}{2}$
 $\lambda_n = \frac{2L}{n}$

 - Frequency is in Hz, fundamental frequency of standing waves is 100 hz, and that scales with the standing wave number. As the standing wave number increases so does the frequency
 - As n increases $\lambda$ decreases and frequency increases
  V = $\lambda f$
  
  F = $\frac{v}{\lambda}$ 
  
 # $F_{n}= V \cdot \frac{1}{\lambda n}$
 
 $F_{n}= \frac{V}{1} \cdot \frac{n}{2L}$

 $F_{n} = nF_1$ 
 - frequency of the harmonic = n $\cdot$ fundamental frequency


nodes = n+1
antinodes = n

# Doppler Effect

$F_{o} = F_{s} \cdot [ \frac{V \pm V_{o}}{V \pm V_{s}}]$

V = 343 m/s = speed of sound

numerator increase = observed frequency increases

denominator increase = observed frequency decreases

 $S ----> observer$
	- $F_0$ increases
	- denominator must decrease
	- so - sign in the denominator
	- 
$S<------          observer$
	- $F_{o}$ increases
	- numerator must increase
	- so + sign in the numerator
$observer <------ S$
	- $F_o$ decreases
	- numerator must decrease
	- so - sign in the numerator




$$

$$







